make set abstract in StateCalculus

src/Common.v
@@ -4,7 +4,7 @@ Require Export compiler.Monad.
 Require Export compiler.Decidable.
 Require Export compiler.Tactics.
 
-Class Map(T K V: Type) := mMap {
+Class Map(T K V: Type) := mkMap {
   empty: T;
   get: T -> K -> option V;
   put: T -> K -> V -> T;
@@ -23,6 +23,24 @@ Instance Function_Map(K V: Type){decK: DecidableEq K}: Map (K -> option V) K V :
 - intros. cbv. destruct_one_match; reflexivity || contradiction.
 - intros. cbv. destruct_one_match; reflexivity || contradiction.
 Defined.
+
+Class set(T E: Type) := mkSet {
+  empty_set: T;
+  singleton_set: E -> T;
+  union: T -> T -> T;
+  intersect: T -> T -> T;
+  contains: T -> E -> Prop;
+}.
+
+Notation "x '\in' s" := (contains s x) (at level 39, no associativity).
+
+Instance Function_Set(E: Type): set (E -> Prop) E := {|
+  empty_set := fun _ => False;
+  singleton_set y := fun x => x = y;
+  union := fun s1 s2 => fun x => s1 x \/ s2 x;
+  intersect := fun s1 s2 => fun x => s1 x /\ s2 x;
+  contains := id
+|}.
 
 Global Instance dec_eq_word : forall sz, DecidableEq (word sz) := weq.
 
